updated it_exec.v; inconsistency problem

proofs/itrees/it_exec.v
@@ -1,3 +1,4 @@
+(*
 From Coq Require Import
      Arith.PeanoNat
      Lists.List
@@ -68,6 +69,9 @@ Local Open Scope option_scope.
 
 Obligation Tactic := done || idtac.
 
+*)
+
+
 (* This files contains the monad transformer associated with exec *)
 
 (*
@@ -88,6 +92,40 @@ About MonadLawsE.
 About mathcomp.ssreflect.seq.
 About result.
 *)
+
+(* begin hide *)
+From Coq Require Import
+  RelationClasses
+  Setoid
+  Morphisms.
+
+From Jasmin Require Import utils. (* expr psem_defs psem oseq. *)
+
+From Paco Require Import paco.
+
+From ITree Require Import
+     Basics.Utils
+     Basics.Basics
+     Basics.Category
+     Basics.CategoryKleisli
+     Basics.HeterogeneousRelations
+     Basics.Monad
+     Core.ITreeDefinition
+     Core.KTree
+     Core.KTreeFacts
+     Eq.Eqit
+     Eq.UpToTaus
+     Eq.Paco2
+     Indexed.Sum
+     Interp.Interp
+     Interp.InterpFacts
+     Interp.RecursionFacts.
+
+Import ITreeNotations.
+Import ITree.Basics.Basics.Monads.
+Local Open Scope itree_scope.
+
+Import Monads.
 
 Section ExecT.
 
@@ -129,6 +167,7 @@ End ExecT.
 
 Section ExecTLaws. 
 
+
 Definition result_rel (W: Set) {X} (R : relation X) (Re : relation W) :
    relation (result W X) :=
 fun (mx my : result W X) =>
@@ -143,8 +182,23 @@ match mx with
           end
 end.
 
-Definition exec_rel {X: Type} (R : relation X) :
+Lemma result_rel_eq (W: Set) : forall {A : Type},
+    eq_rel (@eq (result W A)) (result_rel W eq eq).
+Proof.
+  intros ?; split; intros [] [] EQ; subst; try inv EQ; cbn; auto.
+Qed.
+
+Definition exec_rel' {X: Type} (R : relation X) :
    relation (exec X) := result_rel error R (fun x y => True). 
+
+Definition exec_rel {X: Type} (R : relation X) :
+   relation (exec X) := result_rel error R eq. 
+
+Lemma exec_rel_eq : forall {A : Type},
+    eq_rel (@eq (exec A)) (exec_rel eq).
+Proof.
+  intros ?; split; intros [] [] EQ; subst; try inv EQ; cbn; auto.
+Qed.
 
 (* Universe inconsistency - and can't find a way to fix it *)
 (* Unset Universe Checking.  *)
@@ -162,6 +216,7 @@ Global Instance Symmetric_execT_eq1 {E T} : Symmetric (@execT_Eq1 E T).
     apply Symmetric_eqit.
     unfold Symmetric.
     intros [] [] H; auto; try reflexivity.
+    inv H; reflexivity.
     inv H; reflexivity.
   Qed.
 
@@ -197,3 +252,188 @@ Global Instance MonadLaws_execE {E} : MonadLawsE (execT (itree E)).
   
 End ExecTLaws.
 
+
+Definition interp_exec {E M}
+           {FM : Functor.Functor M} {MM : Monad M}
+           {IM : MonadIter M} (h : E ~> @execT M) :
+  itree E ~> @execT M := interp h.
+Arguments interp_exec {_ _ _ _ _} h [T].
+
+(* (** Unfolding of [interp_fail]. *) *)
+Definition _interp_exec {E F R} (f : E ~> execT (itree F)) (ot : itreeF E R _)
+  : execT (itree F) R :=
+  match ot with
+  | RetF r => ret r
+  | TauF t => Tau (interp_exec f t)
+  | VisF _ e k => bind (f _ e) (fun x => Tau (interp_exec f (k x)))
+  end.
+
+(** Unfold lemma. *)
+Lemma unfold_interp_exec {E F R} (f : E ~> execT (itree F)) (t : itree E R) :
+  interp_exec f t ≅
+         (_interp_exec f (observe t)).
+Proof.
+  unfold interp_exec,interp. unfold Basics.iter, execT_iter, Basics.iter, MonadIter_itree.
+  rewrite unfold_iter. cbn.
+  destruct (observe t).
+  cbn; repeat (rewrite ?bind_bind, ?bind_ret_l, ?bind_map; try reflexivity).
+  cbn; repeat (rewrite ?bind_bind, ?bind_ret_l, ?bind_map; try reflexivity).
+  cbn; repeat (rewrite ?bind_bind, ?bind_ret_l, ?bind_map; try reflexivity).
+  apply eq_itree_clo_bind with (UU := Logic.eq); [reflexivity | intros x ? <-]. 
+  destruct x as [x|].
+  - rewrite bind_ret_l; reflexivity.
+  - rewrite bind_ret_l; reflexivity.
+Qed.
+
+Global Instance interp_exec_eq_itree {X E F} {R : X -> X -> Prop}
+  (h : E ~> execT (itree F)) :
+  Proper (eq_itree R ==> eq_itree (exec_rel R)) (@interp_exec _ _ _ _ _ h X).
+Proof.
+  repeat red. 
+  ginit.
+  pcofix CIH.
+  intros s t EQ.
+  rewrite 2 unfold_interp_exec.
+  punfold EQ; red in EQ.
+  destruct EQ; cbn; subst; try discriminate; pclearbot; try (gstep; constructor; eauto with paco; fail).
+  guclo eqit_clo_bind; econstructor; [reflexivity | intros x ? <-].
+  destruct x as [x|]; gstep; econstructor; eauto with paco itree.
+  unfold exec_rel, result_rel; auto.
+Qed.
+
+(* Convenient special case: [option_rel eq eq] is equivalent to [eq], so we can avoid bothering *)
+Global Instance interp_exec_eq_itree_eq {X E F} (h : E ~> execT (itree F)) :
+  Proper (eq_itree eq ==> eq_itree eq) (@interp_exec _ _ _ _ _ h X).
+Proof.
+  repeat intro.
+  setoid_rewrite result_rel_eq.
+  apply interp_exec_eq_itree; auto.
+Qed.
+
+Global Instance interp_exec_eutt {X E F R} (h : E ~> execT (itree F)) :
+  Proper (eutt R ==> eutt (exec_rel R)) (@interp_exec _ _ _ _ _ h X).
+Proof.
+  repeat red. 
+  einit.
+  ecofix CIH.
+  intros s t EQ.
+  rewrite 2 unfold_interp_exec.
+  punfold EQ; red in EQ.
+  induction EQ; intros; cbn; subst; try discriminate; pclearbot; try (estep; constructor; eauto with paco; fail).
+  - ebind; econstructor; [reflexivity |].
+    intros [] [] EQ; inv EQ.
+    + estep; ebase.
+    + eret.
+    + reflexivity.  
+  - rewrite tau_euttge, unfold_interp_exec; eauto.
+  - rewrite tau_euttge, unfold_interp_exec; eauto.
+Qed.
+
+(* Convenient special case: [option_rel eq eq] is equivalent to [eq], so we can avoid bothering *)
+Global Instance interp_exec_eutt_eq {X E F} (h : E ~> execT (itree F)) :
+  Proper (eutt eq ==> eutt eq) (@interp_exec _ _ _ _ _ h X).
+Proof.
+  repeat intro.
+  rewrite exec_rel_eq.
+  apply interp_exec_eutt; auto.
+Qed.
+
+Lemma interp_exec_tau {E F R} {f : E ~> execT (itree F)} (t: itree E R):
+  eq_itree eq (interp_exec f (Tau t)) (Tau (interp_exec f t)).
+Proof. rewrite unfold_interp_exec. reflexivity. Qed.
+
+Lemma interp_exec_vis {E F : Type -> Type} {T U : Type}
+      (e : E T) (k : T -> itree E U) (h : E ~> execT (itree F)) 
+  : interp_exec h (Vis e k) 
+                ≅ h T e >>= fun mx =>
+                              match mx with
+                              | Error e => Ret (Error e)
+                              | Ok x => Tau (interp_exec h (k x))
+                              end.
+Proof.
+  rewrite unfold_interp_exec. reflexivity.
+Qed.
+
+(* YZ: as with state, there is this tension between "inlining" the monad transformer
+     in order to rewrite at the itree level, and develop the infrastructure to "properly"
+     work in the transformed monad.
+     With the former style, we pay by systematically exposing what should be handled internally
+     (threading the state, checking on failure).
+     With the latter, we need to be more rigorous with the infrastructure.
+ *)
+Lemma interp_exec_Ret : forall {X E F} (h : E ~> execT (itree F)) (x : X),
+    interp_exec h (Ret x) ≅ Ret (Ok _ x).
+Proof.
+  intros; rewrite unfold_interp_exec; reflexivity.
+Qed.
+
+Lemma interp_exec_ret : forall {X E F} (h : E ~> execT (itree F)) (x : X),
+    interp_exec h (Ret x) ≅ ret (m := execT (itree F)) x.
+Proof.
+  intros; rewrite unfold_interp_exec; reflexivity.
+Qed.
+
+Lemma interp_exec_trigger {E F : Type -> Type} {R : Type}
+      (e : E R) (f : E ~> execT (itree F)) 
+  : interp_exec f (ITree.trigger e) ≈ f _ e.
+Proof.
+  unfold ITree.trigger. rewrite interp_exec_vis.
+  match goal with
+    |- ?y ≈ ?x => remember y; rewrite <- (bind_ret_r x); subst
+  end.
+  eapply eutt_eq_bind.
+  intros []; try reflexivity; rewrite interp_exec_ret,tau_eutt.
+  reflexivity.
+Qed.
+
+(* Inlined *)
+Lemma interp_exec_bind : forall {X Y E F} (t : itree _ X) (k : X -> itree _ Y) (h : E ~> execT (itree F)),
+    interp_exec h (ITree.bind t k) ≅
+                ITree.bind (interp_exec h t)
+                (fun mx => match mx with | (Error e) => ret (Error e) | Ok x => interp_exec h (k x) end).
+Proof.
+  intros X Y E F; ginit; pcofix CIH; intros.
+  rewrite unfold_bind.
+  rewrite (unfold_interp_exec h t).
+  destruct (observe t) eqn:EQ; cbn.
+  - rewrite bind_ret_l. apply reflexivity.
+  - cbn. rewrite bind_tau, !interp_exec_tau.
+    gstep. econstructor; eauto with paco.
+  - rewrite bind_bind, interp_exec_vis.
+    guclo eqit_clo_bind; econstructor.
+    reflexivity.
+    intros [] ? <-; cbn.
+    + rewrite bind_tau.
+      gstep; constructor.
+      ITree.fold_subst.
+      auto with paco.
+    + rewrite bind_ret_l.
+      apply reflexivity.
+Qed.
+
+(* proper *)
+Lemma interp_exec_bind' : forall {X Y E F} (t : itree _ X) (k : X -> itree _ Y) (h : E ~> execT (itree F)),
+    interp_exec h (bind t k) ≅
+                bind (interp_exec h t)
+                (fun x => interp_exec h (k x)).
+Proof.
+  intros X Y E F.
+  cbn.
+  ginit; pcofix CIH; intros.
+  cbn in *.
+  rewrite unfold_bind, (unfold_interp_exec _ t).
+  destruct (observe t) eqn:EQ; cbn.
+  - rewrite bind_ret_l. apply reflexivity.
+  - rewrite bind_tau, !interp_exec_tau.
+    gstep. econstructor; eauto with paco.
+  - rewrite bind_bind, interp_exec_vis.
+    guclo eqit_clo_bind; econstructor.
+    reflexivity.
+    intros [] ? <-; cbn.
+    + rewrite bind_tau.
+      gstep; constructor.
+      ITree.fold_subst.
+      auto with paco.
+    + rewrite bind_ret_l.
+      apply reflexivity.
+Qed.
